Work on ctxt_ref def

theories/contextual_refinement.v
@@ -2,25 +2,16 @@ From stdpp Require Import gmap fin_maps fin_sets.
 
 From cap_machine Require Import machine_parameters cap_lang linking machine_run.
 
-
+(** Minimal free memory in which to write our contexts *)
+Definition reserved_context_size: Addr := (za ^+ 100000)%a.
 
 Section contextual_refinement.
   Context `{MachineParameters}.
-
-  Variable b_stk: Addr.
-  Variable e_stk: Addr.
 
   (* Type of symbols to uniquely identify exports/inports. *)
   Variable Symbols : Type.
   Variable Symbols_eq_dec: EqDecision Symbols.
   Variable Symbols_countable: Countable Symbols.
-
-  (** Predicate that states a word can only access addresses in a given set *)
-  Definition can_address_only (word: Word) (addr_set: gset Addr) :=
-    match word with
-    | WInt _ => True
-    | WCap _ b e _ => ∀ a, (b <= a < e)%a -> a ∈ addr_set
-    end.
 
   (** A predicate that must hold on all word of our segments
       Typically that if it is a capability, it only points into the segment
@@ -40,42 +31,52 @@ Section contextual_refinement.
   (** Contextual refinement requires word_restrictions to imply
       that capabilities only point to the given set *)
   Variable word_restrictions_implies_address_only:
-    ∀ w dom, word_restrictions w dom -> can_address_only w dom.
+      ∀ w dom, word_restrictions w dom -> can_address_only w dom.
 
-  #[local] Notation m_pre_component := (pre_component Symbols _ _).
-  #[local] Notation m_component := (component Symbols _ _).
-  #[local] Notation Main := (Main _ _ _).
-  #[local] Notation Lib := (Lib _ _ _).
+  (** A predicate on the addresses used by our components
+      Since memory is finite, we need have some free memory for our contexts
+      otherwise any program that takes the whole memory would refine into anything
 
-  #[local] Notation exports := (exports Symbols _ _).
-  #[local] Notation imports := (imports Symbols _ _).
+      When in doubt, instanciate this with [addr_gt_than reserved_context_size] *)
+  Variable addr_restrictions: gset Addr -> Prop.
 
-  #[local] Notation is_context := (is_context e_stk Symbols _ _ word_restrictions).
-  #[local] Notation link := (link e_stk Symbols _ _ word_restrictions).
+  (** Creating a link requires that addr_restriction remains true on unions *)
+  Variable addr_restrictions_union_stable:
+    forall dom1 dom2,
+      addr_restrictions dom1 ->
+      addr_restrictions dom2 ->
+      addr_restrictions (dom1 ∪ dom2).
 
-  #[local] Notation wf_pre_comp := (well_formed_pre_comp e_stk Symbols _ _ word_restrictions).
-
-  #[local] Notation make_link_main_lib := (make_link_main_lib Symbols _ _).
+  (** Contextual refinement requires addr_restrictions to imply
+      that the first [reserved_context_size] addresses are free *)
+  Variable addr_restrictions_implies_addr_gt:
+    ∀ dom, addr_restrictions dom -> addr_gt_than reserved_context_size dom.
 
   (** Register that holds the stack capability. Any != PC will do
       since we quantify over all programs *)
   Definition r_stk := r_t1.
 
-  Section ctxt_ref_def.
+  Section definition.
 
     (** Component with proof of their well-formedness *)
-    Definition component_wf := { x: m_pre_component | wf_pre_comp x }.
+    Record component_wf := {
+      comp : pre_component Symbols_countable;
+      comp_is_wf : well_formed_pre_comp word_restrictions addr_restrictions comp
+    }.
 
     (** Create a initial machine state from a component:
         - registers are all 0, except PC which is main, and r_stk which points to the stack
         - the memory is the one specified in the segment *)
-    Definition initial_state (c: m_component) :=
+    Definition initial_state (c: component Symbols_countable) :=
       match c with
       | Lib pre_comp => (∅, ∅) (* dummy value *)
-      | Main (ms, _, _) c_main =>
-        (<[r_stk := WCap RWX b_stk e_stk b_stk]>
-        (<[PC := c_main]> (gset_to_gmap (WInt 0) (list_to_set all_registers))), ms)
+      | Main pre_comp c_main =>
+        (<[PC := c_main]> (gset_to_gmap (WInt 0) (list_to_set all_registers)),
+        pre_comp.(segment))
       end.
+
+    Definition unconstrained_addr : gset Addr -> Prop :=
+      fun _ => True.
 
     (** This is the contextual refinement relation
         A component 'impl' contextually refines 'spec' if,
@@ -89,33 +90,36 @@ Section contextual_refinement.
         - 'ctxt' is a valid context to run 'spec'
         - 'ctxt' linked with 'spce' also terminates in 'c' *)
     Definition contextual_refinement : relation component_wf :=
-      fun implementation specification: component_wf =>
-      let impl := proj1_sig implementation in
-      let spec := proj1_sig specification in
-      forall (context: m_pre_component) (main:Word) (c: ConfFlag),
-        let linked_impl := make_link_main_lib context impl main in
-        let linked_spec := make_link_main_lib context spec main in
+      fun impl spec =>
+      forall (context: pre_component Symbols_countable) (main:Word) (c: ConfFlag),
+        let linked_impl := link_main_lib context impl.(comp) main in
+        let linked_spec := link_main_lib context spec.(comp) main in
         let ctxt := Main context main in
-        well_formed_comp e_stk Symbols _ _ word_restrictions ctxt ->
-        is_context ctxt (Lib impl) linked_impl ->
+        well_formed_comp word_restrictions unconstrained_addr ctxt ->
+        is_context word_restrictions unconstrained_addr ctxt (Lib impl.(comp)) linked_impl ->
         (exists n, machine_run n (Executable, initial_state linked_impl) = Some c) ->
-        is_context ctxt (Lib spec) linked_spec /\
+        is_context word_restrictions unconstrained_addr ctxt (Lib spec.(comp)) linked_spec /\
           (exists n, machine_run n (Executable, initial_state linked_spec) = Some c).
-  End ctxt_ref_def.
+  End definition.
 
-  Lemma contextual_reflexive : Reflexive contextual_refinement.
-  Proof.
-    intros [impl impl_wf] context main c linked_impl linked_spec ctxt wf_context is_ctxt1 mr.
-    split; assumption.
-  Qed.
+  Section facts.
 
-  Lemma contextual_transitive : Transitive contextual_refinement.
-  Proof.
-    intros [lib_a a_wf] [lib_b b_wf] [lib_c c_wf] a_b b_c.
-    intros context main c linked_a linked_c ctxt wf_context is_ctxt_a mr_a.
-    destruct (a_b context main c wf_context is_ctxt_a mr_a) as [is_ctxt_b mr_b].
-    apply (b_c context main c wf_context is_ctxt_b mr_b).
-  Qed.
+    (** Contextual refinement is reflexive *)
+    #[global] Instance ctxt_ref_reflexive : Reflexive contextual_refinement.
+    Proof.
+      intros [impl impl_wf] context main c linked_impl linked_spec ctxt wf_context is_ctxt1 mr.
+      split; assumption.
+    Qed.
 
+    (** Contextual refinement is transitive *)
+    #[global] Instance ctxt_ref_transitive : Transitive contextual_refinement.
+    Proof.
+      intros [lib_a a_wf] [lib_b b_wf] [lib_c c_wf] a_b b_c.
+      intros context main c linked_a linked_c ctxt wf_context is_ctxt_a mr_a.
+      destruct (a_b context main c wf_context is_ctxt_a mr_a) as [is_ctxt_b mr_b].
+      apply (b_c context main c wf_context is_ctxt_b mr_b).
+    Qed.
+
+  End facts.
 
 End contextual_refinement.
